type/beta.v
@@ -1,0 +1,487 @@
+From RDST Require Import type.unscoped type.local.
+Require Import String List Datatypes Lia Relations.
+Import ListNotations.
+Local Open Scope string_scope.
+Local Open Scope list_scope.
+Require Import Setoid Morphisms Coq.Program.Basics.
+
+Fixpoint compute_plus (e1 e2: local): option local :=
+  match (e1, e2) with
+    | (ltzero, ltzero)       => Some ltzero
+    | (ltsucc k1, ltsucc k2) => let s := (compute_plus k1 k2) in
+                                match s with
+                                  | Some ss => Some (ltsucc (ltsucc ss))
+                                  | _       => None
+                                end
+    | (ltsucc k1, ltzero)    => Some e1
+    | (ltzero, ltsucc k2)    => Some e2
+    | _                      => None
+  end.
+
+(* Eval compute in compute_plus (ltsend "p" "l" ltnat ltend) (ltsucc (ltsucc ltzero)). *)
+
+Definition complus (e: local): local :=
+  match e with
+    | ltplus e1 e2 =>
+    let fix next e1 e2 :=
+      match (e1, e2) with
+        | (ltzero, ltzero)       => ltzero
+        | (ltsucc k1, ltsucc k2) => (ltsucc (ltsucc (next k1 k2)))
+        | (ltsucc k1, ltzero)    => e1
+        | (ltzero, ltsucc k2)    => e2
+        | _                      => e
+      end
+    in next e1 e2
+    | _           => e
+  end.
+
+(* Eval compute in complus (ltplus  (ltsucc (ltsucc ltzero)) (ltsucc (ltsucc ltzero))). *)
+
+Fixpoint betaP (s: local): local :=
+  match s with
+    | ltapp (ltlambda e1 e2) e3    => subst_local (e3 .: ltvar) e2
+    | ltlambda e1 e2               => ltlambda (betaP e1) (betaP e2)
+    | ltapp (ltpi e1 e2) e3        => subst_local (e3 .: ltvar) e2
+    | ltpi e1 e2                   => ltpi (betaP e1) (betaP e2)
+    | ltsig e1 e2                  => ltsig (betaP e1) (betaP e2)
+    | ltite (lttrue) e1 e2         => e1
+    | ltite (ltfalse) e1 e2        => e2
+    | ltplus e1 e2                 => complus s
+    | _                            => s
+  end.
+
+Fixpoint retRecPath (l: label) (xs: list(label*local*local)): option local :=
+  match xs with
+    | nil             => None
+    | (lbl,t,c) :: ys => if eqb l lbl then Some c else retRecPath l ys
+  end.
+
+Inductive lqueue (p: participant): Type := 
+  | lnil : lqueue p
+  | lcons: participant -> label -> local -> lqueue p -> lqueue p.
+
+Arguments lnil {_}.
+Arguments lcons {_} _ _ _.
+
+Fixpoint lconq {p: participant} (m1 m2: lqueue p): lqueue p :=
+  match m1 with
+    | lnil           => m2
+    | lcons q l c qu => lcons q l c (lconq qu m2)
+  end.
+
+Inductive gqueue: Type :=
+  | gnil : gqueue
+  | gcons: forall p, lqueue p -> gqueue -> gqueue.
+
+Fixpoint genq (p: participant) (q: participant) (l: label) (t: local) (m: gqueue) : gqueue :=
+  match m with
+    | gnil           => gcons p (lcons q l t lnil) gnil
+    | gcons p1 i1 m1 => if eqb p p1 then gcons p1 (lcons q l t i1) m1 else gcons p1 i1 (genq p q l t m1)
+  end.
+
+Definition isNil {p: participant} (l: lqueue p) :=
+  match l with
+    | lnil => true
+    | _    => false
+  end.
+
+Fixpoint gdeq (p: participant) (k: participant) (m: gqueue): option (participant*label*local)*gqueue :=
+  match m with
+    | gnil         => (None,m)
+    | gcons q i m1 => if eqb p q then 
+                        let fix next k i :=
+                          match i with
+                           | lnil           => (None,i)
+                           | lcons r l c i1 => if (eqb r k) then (Some (r,l,c), i1)
+  (*                                              else if isNil i1 then (None, i1)  *)
+                                               else ((fst (next k i1)), lcons r l c (snd (next k i1)))
+                          end
+                          in (let out := (next k i) in (fst out, gcons q (snd out) m1))
+                      else 
+                        let out := (gdeq p k m1) in (fst out, gcons q i (snd out))
+  end.
+
+Class process: Type :=
+  mkproc
+  {
+    body : local;
+    queue: gqueue
+  }.
+
+Fixpoint incn (u: local): local :=
+  match u with
+    | ltmu P t       => ltmu (incn P) t
+    | ltlambda e1 e2 => ltlambda (incn e1) (incn e2)
+    | ltapp e1 e2    => ltapp (incn e1) (incn e2)
+    | ltsubtr e1 e2  => ltsubtr (incn e1) (incn e2)
+    | ltadd e1 e2    => ltadd (incn e1) (incn e2)
+    | ltmult e1 e2   => ltmult (incn e1) (incn e2)
+    | ltgt e1 e2     => ltgt (incn e1) (incn e2)
+    | ltvar 0        => ltvar 0
+    | ltvar (S k)    => ltvar (S (S k))
+    | ltite e1 e2 e3 => ltite (incn e1) (incn e2) (incn e3)
+    | _              => u
+  end.
+
+Fixpoint betaL (u: local): local :=
+  match u with
+    | ltapp (ltlambda e1 e2) e3 => (subst_local (e3 .: ltvar) e2) 
+(*     | ltapp (ltmu e1 e2) e3     => (subst_local (e3 .: ltvar) ((ltmu e1 e2)))  *)
+    | ltapp (ltpi e1 e2) e3     => (subst_local (e3 .: ltvar) e2)
+    | ltite (lttrue) e1 e2      => e1
+    | ltite (ltfalse) e1 e2     => e2 
+    | ltplus e1 e2              => (complus (ltplus e1 e2))
+    | ltmu P t as f             => incn (subst_local (f .: ltvar) P)
+    | ltlambda e1 e2            => ltlambda (betaL e1) (betaL e2)
+    | ltadd e1 e2               => match (e1,e2) with
+                                     | (ltnval n, ltnval m) => ltnval (n+m)
+                                     | _                    => ltadd (betaL e1) (betaL e2) 
+                                   end
+    | ltmult e1 e2              => match (e1,e2) with
+                                     | (ltnval n, ltnval m) => ltnval (n*m)
+                                     | _                    => ltmult (betaL e1) (betaL e2) 
+                                   end
+    | ltsubtr e1 e2             =>  match (e1,e2) with
+                                     | (ltnval n, ltnval m) => ltnval (n-m)
+                                     | _                    => ltsubtr (betaL e1) (betaL e2) 
+                                   end
+    | ltgt e1 e2                => match (e1,e2) with
+                                     | (ltnval n, ltnval m) => ltbval (Nat.ltb m n)
+                                     | _                    => ltgt (betaL e1) (betaL e2) 
+                                   end
+    | ltite e1 e2 e3            => match e1 with
+                                     | ltbval true  => e2
+                                     | ltbval false => e3
+                                     | _            => ltite (betaL e1) e2 e3 
+                                   end
+    | ltapp e1 e2              => ltapp (betaL e1) (betaL e2)
+    | _                        => u
+  end.
+
+Definition beta (k: participant) (u: process): process :=
+  match @body u with
+   | ltsend p l e C             => mkproc C (genq k p l e (@queue u))
+   | ltreceive p xs             => let m := gdeq p k (@queue u) in
+                                    match m with
+                                      | (Some (i1,i2,i3),m') => 
+                                        let t := retRecPath i2 xs in
+                                        match t with
+                                          | Some t' => (mkproc (subst_local (i3 .: ltvar) t') m')
+                                          | None    => u
+                                        end
+                                      | (None,_)             => u
+                                    end
+    | ltbranch p xs             => let m := gdeq p k (@queue u) in
+                                    match m with
+                                      | (Some (i1,i2,i3),m') => 
+                                        let t := retRecPath i2 xs in
+                                        match t with
+                                          | Some t' => (mkproc (subst_local (i3 .: ltvar) t') m')
+                                          | None    => u
+                                        end
+                                      | (None,_)             => u
+                                    end
+    | ltselect p l e C          => (mkproc C (genq k p l e (@queue u)))
+(*     | ltmu (ltlambda e1 e2) t as f => (mkproc (betaL (@body u)) (@queue u)) *)
+    | ltmu P t as f             => (mkproc (subst_local (f .: ltvar) P) (@queue u))
+    | ltapp (ltlambda e1 e2) e3 => (mkproc (subst_local (e3 .: ltvar) e2) (@queue u))
+    | ltapp (ltpi e1 e2) e3     => (mkproc (subst_local (e3 .: ltvar) e2) (@queue u))
+    | ltapp e1 e2 as f          => (mkproc (betaL f) (@queue u))
+    | ltlambda e1 e2 as f       => (mkproc (betaL f) (@queue u))
+    | ltite (lttrue) e1 e2      => (mkproc e1 (@queue u))
+    | ltite (ltfalse) e1 e2     => (mkproc e2 (@queue u))
+    | ltite e1 e2 e3 as f       => (mkproc (betaL f) (@queue u))
+    | ltplus e1 e2              => (mkproc (complus (ltplus e1 e2)) (@queue u))
+    | ltadd e1 e2 as f          => (mkproc (betaL f) (@queue u))
+    | ltmult e1 e2 as f         => (mkproc (betaL f) (@queue u))
+    | ltgt e1 e2 as f           => (mkproc (betaL f) (@queue u))
+    | ltsubtr e1 e2 as f        => (mkproc (betaL f) (@queue u))
+    | _                         => u
+  end.
+
+Definition isVal (s: process): bool :=
+  match (@body s) with
+    | ltlambda e1 e2 => true
+    | ltpi e1 e2     => true
+    | ltstar         => true
+    | ltsucc n       => true
+    | ltzero         => true
+    | _              => false
+  end.
+
+Fixpoint betan (n: nat) (p: participant) (s: process): process :=
+  match n with
+    | O   => s
+    | S k => (* if isVal s then s else  *) betan k p (beta p s) 
+  end.
+
+Definition betanL (n: nat) (p: participant) (s: process): process :=
+  let fix next n b :=
+    match n with
+      | O   => b
+      | S k => next k (betaL b) 
+    end
+  in mkproc (next n (@body s)) (@queue s).
+
+Inductive session: Type :=
+  | sind: participant -> process -> session
+  | spar: session     -> session -> session.
+
+Notation "p '<--' P | h" :=  (sind p (mkproc P h)) (at level 50, no associativity).
+Notation "s1 '|||' s2"   :=  (spar s1 s2) (at level 50, no associativity): type_scope.
+
+Class sessionA: Type :=
+ mksession
+ {
+   und   : session;
+   squeue: gqueue
+ }.
+
+Fixpoint agqueue (m1 m2: gqueue): gqueue :=
+  match m1 with
+    | gnil => m2
+    | gcons p i m => gcons p i (agqueue m m2)
+  end.
+
+Inductive betaS: relation sessionA :=
+  | r_send   : forall p q l p1 c lq gq M, let e1 := (beta p (mkproc (ltsend q l p1 c) lq)) in
+                                          betaS (mksession ((p <-- (ltsend q l p1 c) | lq) ||| M) gq)
+                                                (mksession ((p <-- (@body e1) | (@queue e1)) ||| M) (agqueue (@queue e1) gq))
+  | r_receive: forall p k xs gq lq M, let m := gdeq k p gq in
+                                      let e1 := (beta p (mkproc (ltreceive k xs) gq)) in
+                                      betaS (mksession ((p <-- (ltreceive k xs) | lq) ||| M) gq)
+                                            (mksession ((p <-- (@body e1) | lq) ||| M) (snd m))
+  | r_rest   : forall p p1 lq gq M, let e := (beta p (mkproc p1 lq)) in
+                                    betaS (mksession ((p <-- p1 | lq) ||| M) gq)
+                                          (mksession ((p <-- (@body e) | lq) ||| M) gq).
+
+Definition PAlice: local := 
+  (ltsend "Bob" "l1" (ltzero) (ltreceive "Carol" [("l3",ltnat,ltend)])).
+
+Definition PBob: local :=
+   (ltreceive "Alice" [("l1",ltnat,(ltsend "Carol" "l2" (ltsucc ltzero) ltend));
+                       ("l4",ltnat,(ltsend "Carol" "l2" (ltsucc (ltsucc ltzero)) ltend))
+                      ]).
+
+Definition PCarol: local :=
+ (ltreceive "Bob" [("l2",ltnat,(ltsend "Alice" "l3" (ltplus (ltvar 0) (ltsucc (ltzero))) ltend))]).
+
+
+Definition MS: sessionA := mksession (("Alice" <-- PAlice | gnil) ||| ("Bob" <-- PBob | gnil) ||| ("Carol" <-- PCarol | gnil)) gnil.
+
+Definition MS': sessionA := mksession (("Alice" <-- ltend | (gcons "Alice" (lcons "Bob" "l1" ltzero lnil) gnil)) 
+                                   ||| ("Bob"   <-- ltend | (gcons "Bob" (lcons "Carol" "l2" (ltsucc ltzero) lnil) gnil)) 
+                                   ||| ("Carol" <-- ltend | (gcons "Carol" (lcons "Alice" "l3" (ltplus (ltsucc ltzero) (ltsucc ltzero)) lnil) gnil)))
+                                   (gcons "Carol" lnil (gcons "Bob" lnil (gcons "Alice" lnil gnil))).
+
+Inductive pcong: relation local :=
+  | pmuUnf: forall e p, pcong (ltmu e p) (subst_local ((ltmu e p) .: (ltvar)) p).
+
+Inductive lqcong {p: participant}: relation (lqueue p) :=
+  | qcons : forall q1 q2 l1 l2 v1 v2 h1 h2, q1 <> q2 -> 
+                                            lqcong (lconq h1 (lconq (lcons q1 l1 v1 lnil) (lconq (lcons q2 l2 v2 lnil) h2)))
+                                                   (lconq h1 (lconq (lcons q2 l2 v2 lnil) (lconq (lcons q1 l1 v1 lnil) h2))).
+
+Inductive scongA: relation sessionA :=
+  | srecA   : forall p P e hp h M, scongA (mksession ((p <-- (ltmu P e) | hp) ||| M) h) (mksession ((p <-- (subst_local ((ltmu P e) .: ltvar) P) | hp) ||| M) h)
+  | sannA   : forall p M h, scongA (mksession ((p <--  ltend | gnil) ||| M) h) (mksession M h)
+  | scommA  : forall M1 M2 h, scongA (mksession (M1 ||| M2) h) (mksession (M2 ||| M1) h)
+  | sassocA : forall M1 M2 M3 h, scongA (mksession (M1 ||| M2 ||| M3) h) (mksession (M1 ||| (M2 ||| M3)) h)
+(*   | sassoc2: forall M1 M2 M3, scong (M1 ||| M2 ||| M3) ((M1 ||| M2) ||| M3) *)
+  | sassoc2A: forall M1 M2 M3 h, scongA (mksession (M1 ||| M2 ||| M3) h) (mksession (M1 ||| (M3 ||| M2)) h).
+
+Inductive scong: relation session :=
+  | sann   : forall p M, scong ((p <--  ltend | gnil) ||| M) M
+  | scomm  : forall M1 M2, scong (M1 ||| M2) (M2 ||| M1)
+  | sassoc : forall M1 M2 M3, scong (M1 ||| M2 ||| M3) (M1 ||| (M2 ||| M3))
+(*   | sassoc2: forall M1 M2 M3, scong (M1 ||| M2 ||| M3) ((M1 ||| M2) ||| M3) *)
+  | sassoc2: forall M1 M2 M3, scong (M1 ||| M2 ||| M3) (M1 ||| (M3 ||| M2)).
+(*   | scongl : forall p P Q h1 h2 M, pcong P Q -> lqcong h1 h2 -> 
+                                   scong ((p <-- (mkproc P h1)) ||| M) ((p <-- (mkproc Q h2)) ||| M). *)
+
+Declare Instance Equivalence_beta : Equivalence betaS.
+Declare Instance Equivalence_scong : Equivalence scong.
+Declare Instance Equivalence_scongA : Equivalence scongA.
+
+Inductive multi {X : Type} (R : relation X) : relation X :=
+  | multi_refl : forall (x : X), multi R x x
+  | multi_step : forall (x y z : X), R x y -> multi R y z -> multi R x z.
+
+Definition betaS_multistep := multi betaS.
+
+#[global] Declare Instance RW_scong2: Proper (scongA ==> scong) (@und).
+
+#[global] Declare Instance RW_scong3: Proper (scongA ==> scongA ==> impl) betaS.
+#[global] Declare Instance RW_scong4: Proper (scongA ==> scongA ==> impl) betaS_multistep.
+
+Example redMS: betaS_multistep MS MS'.
+Proof. intros.
+       unfold betaS_multistep, MS, MS', PAlice.
+
+       (* Eval compute in (beta "Alice" 
+                              (mkproc (ltsend "Bob" "l1" ltzero (ltreceive "Carol" [("l3", ltnat, ltend)]))
+                              gnil)). *)
+
+       (* Eval compute in (beta "Bob" 
+                              (mkproc (ltreceive "Alice" [("l1", ltnat, ltsend "Carol" "l2" (ltsucc ltzero) ltend);
+                                                          ("l4", ltnat, ltsend "Carol" "l2" (ltsucc (ltsucc ltzero)) ltend)])
+                               gnil)). *)
+
+       apply multi_step with
+       (y :=  mksession ((("Alice" <-- ltreceive "Carol" [("l3", ltnat, ltend)] | ( gcons "Alice" (lcons "Bob" "l1" ltzero lnil) gnil))
+                      ||| ("Bob" <-- PBob | gnil))
+                      ||| ("Carol" <-- PCarol | gnil)) (gcons "Alice" (lcons "Bob" "l1" ltzero lnil) gnil)).
+       specialize(r_send "Alice" "Bob" "l1" 
+                         ltzero
+                         (ltreceive "Carol" [("l3", ltnat, ltend)])
+                         gnil
+                         gnil
+                         (("Bob" <-- PBob | gnil) ||| ("Carol" <-- PCarol | gnil))
+       ); intro HS.
+       simpl in HS.
+       setoid_rewrite sassocA.
+       apply HS.
+
+       setoid_rewrite sassocA.
+       setoid_rewrite scommA.
+       unfold PBob.
+
+       (* Eval compute in  (beta "Bob"
+                              (mkproc (ltreceive "Alice" [("l1", ltnat, ltsend "Carol" "l2" (ltsucc ltzero) ltend);
+                                                          ("l4", ltnat, ltsend "Carol" "l2" (ltsucc (ltsucc ltzero)) ltend)])
+                              (gcons "Alice" (lcons "Bob" "l1" ltzero lnil) gnil))). *)
+
+       apply multi_step with
+       (y := mksession ((("Bob" <-- ltsend "Carol" "l2" (ltsucc ltzero) ltend | gnil)
+              ||| ("Carol" <-- PCarol | gnil))
+              ||| ("Alice" <-- ltreceive "Carol" [("l3", ltnat, ltend)] | (gcons "Alice" (lcons "Bob" "l1" ltzero lnil) gnil))) (gcons "Alice" lnil gnil) ).
+
+       specialize(r_receive "Bob" "Alice"
+                            ([("l1", ltnat, ltsend "Carol" "l2" (ltsucc ltzero) ltend);
+                             ("l4", ltnat, ltsend "Carol" "l2" (ltsucc (ltsucc ltzero)) ltend)])
+                            (gcons "Alice" (lcons "Bob" "l1" ltzero lnil) gnil)
+                            gnil
+                            (("Carol" <-- PCarol | gnil) ||| ("Alice" <-- ltreceive "Carol" [("l3", ltnat, ltend)] | (gcons "Alice" (lcons "Bob" "l1" ltzero lnil) gnil)))
+       ); intros HR; simpl in HR.
+       setoid_rewrite sassocA.
+       apply HR.
+
+       unfold PCarol.
+
+       (* Eval compute in (beta "Bob"
+                              (mkproc (ltsend "Carol" "l2" (ltsucc ltzero) ltend) 
+                              gnil)). *)
+
+       apply multi_step with
+       (y := mksession ((("Bob" <-- ltend | (gcons "Bob" (lcons "Carol" "l2" (ltsucc ltzero) lnil) gnil))
+              ||| ("Carol" <-- ltreceive "Bob" [("l2", ltnat, ltsend "Alice" "l3" (ltplus (ltvar 0) (ltsucc ltzero)) ltend)] | gnil))
+              ||| ("Alice" <-- ltreceive "Carol" [("l3", ltnat, ltend)] | gcons "Alice" (lcons "Bob" "l1" ltzero lnil) gnil)) 
+               (gcons "Bob" (lcons "Carol" "l2" (ltsucc ltzero) lnil) (gcons "Alice" lnil gnil)) ).
+
+       specialize(r_send "Bob" "Carol" "l2"
+                         (ltsucc ltzero) 
+                         ltend
+                         gnil
+                         (gcons "Alice" lnil gnil)
+                         (("Carol" <-- ltreceive "Bob" [("l2", ltnat, ltsend "Alice" "l3" (ltplus (ltvar 0) (ltsucc ltzero)) ltend)] | gnil)
+                          ||| ("Alice" <-- ltreceive "Carol" [("l3", ltnat, ltend)] | gcons "Alice" (lcons "Bob" "l1" ltzero lnil) gnil))
+       ); intro HR; simpl in HR.
+        setoid_rewrite sassocA.
+        apply HR.
+
+       setoid_rewrite sassocA.
+       setoid_rewrite scommA.
+       setoid_rewrite sassoc2A.
+
+
+       (* Eval compute in (beta "Carol"
+                              (mkproc (ltreceive "Bob" [("l2", ltnat, ltsend "Alice" "l3" (ltplus (ltvar 0) (ltsucc ltzero)) ltend)]) 
+                              (gcons "Bob" (lcons "Carol" "l2" (ltsucc ltzero) lnil) (gcons "Alice" lnil gnil)))). *)
+
+       apply multi_step with
+       (y := mksession ((("Carol" <-- ltsend "Alice" "l3" (ltplus (ltsucc ltzero) (ltsucc ltzero)) ltend | gnil)
+              ||| ("Bob" <-- ltend | gcons "Bob" (lcons "Carol" "l2" (ltsucc ltzero) lnil) gnil))
+              ||| ("Alice" <-- ltreceive "Carol" [("l3", ltnat, ltend)] | gcons "Alice" (lcons "Bob" "l1" ltzero lnil) gnil)) 
+               (gcons "Bob" lnil (gcons "Alice" lnil gnil)) ).
+       specialize(r_receive "Carol" "Bob"
+                            ([("l2", ltnat, ltsend "Alice" "l3" (ltplus (ltvar 0) (ltsucc ltzero)) ltend)])
+                            (gcons "Bob" (lcons "Carol" "l2" (ltsucc ltzero) lnil) (gcons "Alice" lnil gnil))
+                            gnil
+       ); intro HR; simpl in HR.
+       setoid_rewrite sassocA.
+       apply HR.
+
+       (*  Eval compute in (beta "Carol" 
+                                 (mkproc (ltsend "Alice" "l3" (ltplus (ltsucc ltzero) (ltsucc ltzero)) ltend)  
+                                 (gnil))). *)
+
+       setoid_rewrite sassoc2A.
+
+       apply multi_step with
+       (y := mksession ((("Carol" <-- ltend | (gcons "Carol" (lcons "Alice" "l3" (ltplus (ltsucc ltzero) (ltsucc ltzero)) lnil) gnil))
+              ||| ("Alice" <-- ltreceive "Carol" [("l3", ltnat, ltend)] | gcons "Alice" (lcons "Bob" "l1" ltzero lnil) gnil))
+              ||| ("Bob" <-- ltend | gcons "Bob" (lcons "Carol" "l2" (ltsucc ltzero) lnil) gnil)) 
+               (gcons "Carol" (lcons "Alice" "l3" (ltplus (ltsucc ltzero) (ltsucc ltzero)) lnil) (gcons "Bob" lnil (gcons "Alice" lnil gnil))) ).
+
+       specialize(r_send "Carol" "Alice" "l3"
+                         (ltplus (ltsucc ltzero) (ltsucc ltzero))
+                         ltend
+                         gnil
+                         (gcons "Bob" lnil (gcons "Alice" lnil gnil))
+                         ((("Alice" <-- ltreceive "Carol" [("l3", ltnat, ltend)] | gcons "Alice" (lcons "Bob" "l1" ltzero lnil) gnil)
+                          ||| ("Bob" <-- ltend | gcons "Bob" (lcons "Carol" "l2" (ltsucc ltzero) lnil) gnil)))
+       ); intro HS; simpl in HS.
+       setoid_rewrite sassocA.
+       apply HS.
+
+       setoid_rewrite sassocA.
+       setoid_rewrite scommA.
+       setoid_rewrite sassoc2A.
+
+       (* Eval compute in (beta "Alice" 
+                             (mkproc (ltreceive "Carol" [("l3", ltnat, ltend)])
+                             (gcons "Carol" (lcons "Alice" "l3" (ltplus (ltsucc ltzero) (ltsucc ltzero)) lnil) (gcons "Bob" lnil (gcons "Alice" lnil gnil))))). *)
+
+       apply multi_step with
+       (y := mksession ((("Alice" <-- ltend | gcons "Alice" (lcons "Bob" "l1" ltzero lnil) gnil)
+              ||| ("Carol" <-- ltend | gcons "Carol" (lcons "Alice" "l3" (ltplus (ltsucc ltzero) (ltsucc ltzero)) lnil) gnil))
+              ||| ("Bob" <-- ltend | gcons "Bob" (lcons "Carol" "l2" (ltsucc ltzero) lnil) gnil)) 
+               (gcons "Carol" lnil (gcons "Bob" lnil (gcons "Alice" lnil gnil))) ).
+       specialize(r_receive "Alice" "Carol"
+                            ([("l3", ltnat, ltend)])
+                            (gcons "Carol" (lcons "Alice" "l3" (ltplus (ltsucc ltzero) (ltsucc ltzero)) lnil)
+                              (gcons "Bob" lnil (gcons "Alice" lnil gnil)))
+                            (gcons "Alice" (lcons "Bob" "l1" ltzero lnil) gnil)
+       ); intro HR; simpl in HR.
+       setoid_rewrite sassocA.
+       apply HR.
+
+       setoid_rewrite sassocA.
+       setoid_rewrite scommA.
+       setoid_rewrite sassoc2A at 2.
+       setoid_rewrite sassocA.
+
+       apply multi_refl.
+Qed.
+
+(* factorial example *)
+
+Definition fact: local :=
+  ltmu(
+    ltlambda ltnat (ltite 
+                    (ltgt (ltvar 1) (ltnval 1)) 
+                    (ltmult (ltvar 1) (ltapp (ltvar 0) (ltsubtr (ltvar 1) (ltnval 1)))) 
+                    (ltnval 1)
+                   )
+      ) (ltpi ltnat ltnat).
+
+Definition factorial  (n: nat): local   := ltapp fact (ltnval n).
+Definition pfactorial (n: nat): process := mkproc (factorial n) gnil.
+
+Eval compute in (betan 34 "p" (pfactorial 7)).
+
+
+
+
+
+
