type/typecheck.v
@@ -1,0 +1,56 @@
+From RDST Require Import type.unscoped type.local type.beta.
+Require Import String List Datatypes Lia Relations.
+Import ListNotations.
+Local Open Scope string_scope.
+Local Open Scope list_scope.
+Require Import Setoid Morphisms Coq.Program.Basics.
+From mathcomp Require Import ssreflect.seq.
+
+Fixpoint lookup (c: (list (nat*local))) (m: nat): option local :=
+  match c with
+    | (pair n s1) :: xs => if Nat.eqb n m then Some s1 else lookup xs m
+    |  nil              => None
+  end.
+
+Print process.
+
+Inductive propcont: local -> Prop :=
+  | pc_inact: propcont ltinact
+  | pc_send : forall p l s c, propcont c -> propcont (ltsend p l s c)
+  | pc_recv : forall p C, List.Forall (fun u => propcont u) (map snd C) -> 
+                          propcont (ltreceive p C).
+
+(* incomplete set of rules *)
+Inductive typeCheck: list (fin*local) -> fin -> local -> local -> Prop :=
+  | tc_inact : forall m c, typeCheck c m (ltinact) (ltend)
+  | tc_var  : forall m c s t, Some t = lookup c s ->
+                              typeCheck c m (ltvar s) t
+  | tc_lambda: forall c p k e t' n m, typeCheck c m p ltstar ->
+                                      let t := betan n k (mkproc p gnil) in
+                                      (* ctx ext *)
+                                      typeCheck ((m, (@body t)) :: c) (S m) e t' ->
+                                      typeCheck c m (ltlambda p e) (ltpi (@body t) t')
+  | tc_mu    : forall m c p t, typeCheck ((m, t) :: c) (S m) p t ->
+                               typeCheck c m (ltmu t p) t
+  | tc_app   : forall c k e e' t t' n m, typeCheck c m e (ltpi t t') ->
+                                         typeCheck c m e' t ->
+                                         let tt := subst_local (e' .: ltvar) t' in
+                                         let t'' := betan n k (mkproc tt gnil) in
+                                         typeCheck c m (ltapp e e') (@body t'')
+  | tc_pi    : forall c k p p' (t: local) n m, typeCheck c m p ltstar ->
+                                               let t := betan n k (mkproc p gnil) in
+                                               (* ctx ext *)
+                                               typeCheck ((m, (@body t)) :: c) (S m) p' ltstar ->
+                                               typeCheck c m (ltpi p p') ltstar
+  | tc_send  : forall m c p l e P S T, propcont P ->
+                                       typeCheck c m e S ->
+                                       typeCheck c m P T ->
+                                       typeCheck c m (ltsend p l e P) (ltselect p l S T)
+  | tc_recv  : forall m c p L (ST P T: list local),
+                      List.Forall (fun u => propcont u) P -> 
+                      length L = length ST ->
+                      length ST = length P ->
+                      length P = length T ->
+                      (* ctx ext *)
+                      List.Forall (fun u => typeCheck ((m, (fst u)) :: c) (S m) (fst (snd u)) (snd (snd u))) (zip ST (zip P T)) ->
+                      typeCheck c m (ltreceive p (zip (zip L ST) P)) (ltbranch p (zip (zip L ST) T)).
